Pop/Pop.lean
@@ -5,38 +5,38 @@ open Util
 
 namespace Pop
 
-variable {ArchReqType : Type 0} [BEq ArchReqType] [Inhabited ArchReqType]
+variable [ArchReq]
 
 inductive Transition
-  | acceptRequest : @BasicRequest ArchReqType → ThreadId → Transition
+  | acceptRequest : BasicRequest → ThreadId → Transition
   | propagateToThread : RequestId → ThreadId → Transition
   | satisfyRead : RequestId → RequestId → Transition
  deriving BEq
 
-instance : Inhabited (@Transition ArchReqType) where default := Transition.acceptRequest default 0
+instance : Inhabited (Transition) where default := Transition.acceptRequest default 0
 
-def Transition.toString : @Transition ArchReqType → String
+def Transition.toString : Transition → String
  | acceptRequest req tid => s!"Accept (T{tid}): {req}"
  | propagateToThread reqid tid => s!"Propagate Request {reqid} to Thread {tid}"
  | satisfyRead readid writeid => s!"Satisify Read Request {readid} with Write Request {writeid}"
-instance : ToString (@Transition ArchReqType) where toString := Transition.toString
+instance : ToString (Transition) where toString := Transition.toString
 
-def Transition.isAccept : @Transition ArchReqType → Bool
+def Transition.isAccept : Transition → Bool
  | acceptRequest _ _ => true
  | _ => false
 
-def Transition.isPropagate : @Transition ArchReqType → Bool
+def Transition.isPropagate : Transition → Bool
   | propagateToThread _ _ => true
   | _ => false
 
-def Transition.isSatisfy : @Transition ArchReqType → Bool
+def Transition.isSatisfy : Transition → Bool
   | satisfyRead _ _ => true
   | _ => false
 
-def SystemState.canAcceptRequest : @SystemState ArchReqType → @BasicRequest ArchReqType → ThreadId → Bool
+def SystemState.canAcceptRequest : SystemState → BasicRequest → ThreadId → Bool
  | _, _, _ => true
 
-def SystemState.updateOrderConstraintsPropagate (state : @SystemState ArchReqType) : @Scope state.system.scopes →
+def SystemState.updateOrderConstraintsPropagate (state : SystemState) : @Scope state.system.scopes →
 RequestId → ThreadId → @OrderConstraints state.system.scopes
   | scope, reqId, thId =>
   /-
@@ -68,7 +68,7 @@ RequestId → ThreadId → @OrderConstraints state.system.scopes
       --dbg_trace s!"new constraints: {newConstraints}"
       state.orderConstraints.add_subscopes scope newConstraints
 
-def SystemState.updateOrderConstraintsAccept (state : @SystemState ArchReqType) : @Request ArchReqType → @OrderConstraints state.system.scopes
+def SystemState.updateOrderConstraintsAccept (state : SystemState) : Request → @OrderConstraints state.system.scopes
   | req =>
     let seen := state.idsToReqs state.seen |>.filter (Request.propagatedTo . req.thread)
     let scope := state.system.requestScope req
@@ -77,7 +77,7 @@ def SystemState.updateOrderConstraintsAccept (state : @SystemState ArchReqType) 
     --dbg_trace s!"seen: {seen}, new: {newReqs}"
     state.orderConstraints.add_subscopes scope newConstraints
 
-def SystemState.freshId : @SystemState ArchReqType → RequestId
+def SystemState.freshId : SystemState → RequestId
   | state =>
     let removed := state.removed.map Request.id
     let active := reqIds state.requests
@@ -87,7 +87,7 @@ def SystemState.freshId : @SystemState ArchReqType → RequestId
       | none => 0
       | some id => (Nat.succ id)
 
-def SystemState.applyAcceptRequest : @SystemState ArchReqType → @BasicRequest ArchReqType → ThreadId → @SystemState ArchReqType
+def SystemState.applyAcceptRequest : SystemState → BasicRequest → ThreadId → SystemState
   | state, reqType, tId =>
   let req : Request := { propagated_to := [tId], thread := tId, basic_type := reqType, id := state.freshId}
   --dbg_trace s!"accepting {req}, requests.val : {state.requests.val}"
@@ -102,7 +102,7 @@ def SystemState.applyAcceptRequest : @SystemState ArchReqType → @BasicRequest 
     satisfiedCoherent := sorry
   }
 
-def SystemState.canUnapplyRequest : @SystemState ArchReqType → RequestId → Bool
+def SystemState.canUnapplyRequest : SystemState → RequestId → Bool
   | state, rId =>
   match state.requests.getReq? rId with
    | none => false
@@ -112,7 +112,7 @@ def SystemState.canUnapplyRequest : @SystemState ArchReqType → RequestId → B
      let prop := req.propagated_to == [req.thread]
      succ && prop
 
-def SystemState.unapplyAcceptRequest : @SystemState ArchReqType → RequestId → @SystemState ArchReqType
+def SystemState.unapplyAcceptRequest : SystemState → RequestId → SystemState
 -- TODO: PR for multiple updates?
   | state, rId => {requests := state.requests.remove rId,
                    seen := state.seen, removed := state.removed, orderConstraints := state.orderConstraints,
@@ -127,10 +127,10 @@ def SystemState.unapplyAcceptRequest : @SystemState ArchReqType → RequestId �
 --       let prop := req.propagatedTo thId
 --       -- ...
 
-def Request.isPropagated : @Request ArchReqType → ThreadId → Bool
+def Request.isPropagated : Request → ThreadId → Bool
   | req, thId => req.propagated_to.elem thId
 
-def SystemState.canPropagate : @SystemState ArchReqType → RequestId → ThreadId → Bool
+def SystemState.canPropagate : SystemState → RequestId → ThreadId → Bool
   | state, reqId, thId =>
   match state.requests.getReq? reqId with
   | none => false
@@ -148,13 +148,13 @@ def SystemState.canPropagate : @SystemState ArchReqType → RequestId → Thread
     --dbg_trace s!"R{req.id} unpropagated (T{thId}): {unpropagated}, predPropagated: {predPropagated}"
     unpropagated && predPropagated.foldl (. && .) true
 
-def Request.propagate : @Request ArchReqType → ThreadId → @Request ArchReqType
+def Request.propagate : Request → ThreadId → Request
   | req, thId =>
     let sorted := (thId :: req.propagated_to).toArray.qsort (λ x y => Nat.ble x y)
     { req with propagated_to := sorted.toList}
 
 
-def SystemState.propagate : @SystemState ArchReqType → RequestId → ThreadId → @SystemState ArchReqType
+def SystemState.propagate : SystemState → RequestId → ThreadId → SystemState
   | state, reqId, thId =>
   match state.requests.getReq? reqId with
   | none => state
@@ -168,7 +168,7 @@ def SystemState.propagate : @SystemState ArchReqType → RequestId → ThreadId 
       satisfiedCoherent := state.satisfiedCoherent
     }
 
-def SystemState.canSatisfyRead : @SystemState ArchReqType → RequestId → RequestId → Bool
+def SystemState.canSatisfyRead : SystemState → RequestId → RequestId → Bool
   | state, readId, writeId =>
   if (state.satisfied.map λ x => x.1).elem readId then false else
   match state.requests.val[readId.toNat]?, state.requests.val[writeId.toNat]? with
@@ -187,7 +187,7 @@ def SystemState.canSatisfyRead : @SystemState ArchReqType → RequestId → Requ
         oc && writesToAddrBetween.length == 0
     | _, _ => false
 
-def SystemState.satisfy : @SystemState ArchReqType → RequestId → RequestId → @SystemState ArchReqType
+def SystemState.satisfy : SystemState → RequestId → RequestId → SystemState
  | state, readId, writeId =>
  let opRead := state.requests.getReq? readId
  let opWrite := state.requests.getReq? writeId
@@ -206,31 +206,31 @@ def SystemState.satisfy : @SystemState ArchReqType → RequestId → RequestId �
    | _, _ => unreachable!
 
 open Transition in
-def SystemState.applyTransition! : @SystemState ArchReqType → @Transition ArchReqType → @SystemState ArchReqType
+def SystemState.applyTransition! : SystemState → Transition → SystemState
    | state, (.acceptRequest req tId) => state.applyAcceptRequest req tId
    | state, .propagateToThread reqId tId => state.propagate reqId tId
    | state, satisfyRead readId writeId => state.satisfy readId writeId
 
 open Transition in
-def SystemState.canApplyTransition : @SystemState ArchReqType → @Transition ArchReqType → Bool
+def SystemState.canApplyTransition : SystemState → Transition → Bool
   | state, .acceptRequest req tId => state.canAcceptRequest req tId
   | state, .propagateToThread reqId tId => state.canPropagate reqId tId
   | state, satisfyRead readId writeId => state.canSatisfyRead readId writeId
 
 open Transition in
-def SystemState.applyTransition : @SystemState ArchReqType → @Transition ArchReqType → Except String (@SystemState ArchReqType)
+def SystemState.applyTransition : SystemState → Transition → Except String (SystemState)
   | state, t =>
     if state.canApplyTransition t
     then Except.ok $ state.applyTransition! t
     else throw s!"Invalid transition {t}."
 
-def SystemState.applyTrace : @SystemState ArchReqType → List (@Transition ArchReqType) → Except String (@SystemState ArchReqType)
+def SystemState.applyTrace : SystemState → List (Transition) → Except String (SystemState)
   | state, transitions => transitions.foldlM SystemState.applyTransition state
 
-def SystemState.applyTrace! : @SystemState ArchReqType → List (@Transition ArchReqType) → @SystemState ArchReqType
+def SystemState.applyTrace! : SystemState → List (Transition) → SystemState
   | state, transitions => transitions.foldl SystemState.applyTransition! state
 
-def printResult : Except String (@SystemState ArchReqType) → String
+def printResult : Except String (SystemState) → String
  | Except.ok state => state.toString
  | Except.error e => s!"Error: {e}"
 
